theories/program_logic/proofmode_classes.v
@@ -1,0 +1,84 @@
+From iris.proofmode Require Import base proofmode classes.
+From iris.base_logic.lib Require Export fancy_updates.
+(* From iris.program_logic Require Export language. *)
+(* FIXME: If we import iris.bi.weakestpre earlier texan triples do not
+   get pretty-printed correctly. *)
+From iris.bi Require Export weakestpre.
+From iris.prelude Require Import options.
+From program_logic Require Import state_interpretation weakest_precondition basic_reasoning_rules.
+Import uPred.
+
+(** Proofmode class instances *)
+Section proofmode_classes.
+  Context `{!heapGS Σ}.
+  Implicit Types P Q : iProp Σ.
+  Implicit Types Φ : val → iProp Σ.
+  Implicit Types v : val .
+  Implicit Types e : expr .
+
+  Global Instance frame_wp p s E e R Φ Ψ :
+    (∀ v, Frame p R (Φ v) (Ψ v)) →
+    Frame p R (WP e @ s; E {{ Φ }}) (WP e @ s; E {{ Ψ }}) | 2.
+  Proof. rewrite /Frame=> HR. rewrite wp_frame_l. apply wp_mono, HR. Qed. 
+
+  Global Instance is_except_0_wp s E e Φ : IsExcept0 (WP e @ s; E {{ Φ }}).
+  Proof. by rewrite /IsExcept0 -{2}fupd_wp -except_0_fupd -fupd_intro. Qed.
+
+  Global Instance elim_modal_bupd_wp p E e P Φ :
+    TCEq (to_eff e) None → 
+    ElimModal True p false (|==> P) P (EWP e @ E {{ Φ }}) (EWP e @ E {{ Φ }}).
+  Proof.
+    intros HEq.
+    by rewrite /ElimModal intuitionistically_if_elim
+      (bupd_fupd E) fupd_frame_r wand_elim_r fupd_ewp.
+  Qed.
+
+  Global Instance elim_modal_fupd_wp p E e P Φ :
+    TCEq (to_eff e) None → 
+    ElimModal True p false (|={E}=> P) P (EWP e @ E {{ Φ }}) (EWP e @ E {{ Φ }}).
+  Proof.
+    intros HEq.
+    by rewrite /ElimModal intuitionistically_if_elim
+      fupd_frame_r wand_elim_r fupd_ewp.
+  Qed.
+
+  Global Instance elim_modal_fupd_wp_atomic p E1 E2 e P Φ :
+    TCEq (to_eff e) None → 
+    ElimModal (Atomic StronglyAtomic e) p false
+            (|={E1,E2}=> P) P
+            (EWP e @ E1 {{ Φ }}) (EWP e @ E2 {{ v, |={E2,E1}=> Φ v }})%I | 100.
+  Proof.
+    intros ??. rewrite intuitionistically_if_elim
+      fupd_frame_r wand_elim_r. by apply ewp_atomic.
+  Qed.
+
+  Global Instance add_modal_fupd_wp E e P Φ :
+    TCEq (to_eff e) None → 
+    AddModal (|={E}=> P) P (EWP e @ E {{ Φ }}).
+  Proof. intros ?. by rewrite /AddModal fupd_frame_r wand_elim_r fupd_ewp. Qed.
+
+  Global Instance elim_acc_wp_atomic {X} E1 E2 α β γ e Φ :
+    TCEq (to_eff e) None → 
+    ElimAcc (X:=X) (Atomic StronglyAtomic e)
+            (fupd E1 E2) (fupd E2 E1)
+            α β γ (EWP e @ E1 {{ Φ }})
+            (λ x, EWP e @ E2 {{ v, |={E2}=> β x ∗ (γ x -∗? Φ v) }})%I | 100.
+  Proof.
+    iIntros (??) "Hinner >Hacc".
+    iDestruct "Hacc" as (x) "[Hα Hclose]".
+    iApply (ewp_mono with "(Hinner Hα)").
+    iIntros (v) ">[Hβ HΦ]". iApply "HΦ". by iApply "Hclose".
+  Qed.
+
+  Global Instance elim_acc_wp_nonatomic {X} E α β γ e s Φ :
+    TCEq (to_eff e) None → 
+    ElimAcc (X:=X) True (fupd E E) (fupd E E)
+            α β γ (WP e @ s; E {{ Φ }})
+            (λ x, WP e @ s; E {{ v, |={E}=> β x ∗ (γ x -∗? Φ v) }})%I.
+  Proof.
+    iIntros (? _) "Hinner >Hacc". iDestruct "Hacc" as (x) "[Hα Hclose]".
+    iApply wp_fupd.
+    iApply (wp_wand with "(Hinner Hα)").
+    iIntros (v) ">[Hβ HΦ]". iApply "HΦ". by iApply "Hclose".
+  Qed.
+End proofmode_classes.
