theories/program_logic/reasoning_rules.v
@@ -2,5 +2,7 @@
 
 From program_logic Require Export protocols weakest_precondition
                                   basic_reasoning_rules state_reasoning
+                                  state_interpretation
                                   shallow_handler_reasoning tactics
-                                  deep_handler_reasoning.
+                                  deep_handler_reasoning
+                                  atomics proofmode_classes.
