theories/tests/invariant_test_hazel.v
@@ -7,6 +7,7 @@ From program_logic Require Import reasoning_rules.
 Section name.
 Context `{!heapGS Σ}.
 
+
 Definition invN : namespace := nroot .@ "inv".
 
 Definition inner (l: loc): iProp Σ := ∃ n, l ↦ n.
@@ -31,26 +32,44 @@ Lemma ewp_setone (l: loc):
   MyInv l ⊢ EWP (setone #l) {{_, True}}.
 Proof.
   iIntros "HInv". rewrite /setone. ewp_pure_steps.
+  iInv "HInv" as (n) "Hl" .
+  iApply (ewp_store with "Hl"). iIntros "!> Hl !>!>".
+  iSplit; last done.
+  iNext. iExists #1. done.
+Restart.
+  iIntros "HInv". rewrite /setone. ewp_pure_steps.
   rewrite /MyInv /inner.
-  assert (H: Atomic StronglyAtomic (Store (LitV l) (LitV (Zpos xH)))).
-    by apply _.
-  iApply (@ewp_atomic _ _ ⊤ (⊤ ∖ ↑invN) (Store (LitV l) (LitV (Zpos xH))) _ _ _ H). 
-  iMod (inv_acc with "HInv") as "((%n & Hl) & Hclose)".
-  done.
-  iModIntro.
+  iInv "HInv" as (n) "Hl" "Hclose".
   iApply (ewp_store with "Hl").
+  (* the update modality here is mask-changing
+    i.e. two different masks. So we cannot intros it.
+    Instead, we need to change it to a non-mask-changing update using Hclose. 
+    This is done with the FUP-CHANGE-MASK rule in "Iris from the ground up".
+    Which is apparently fupd_elim in coq *)
   iIntros "!> Hl !>".
-  iApply (fupd_elim (⊤ ∖ ↑invN) ⊤ ⊤ True True).
-    by iIntros "_ !>". 
   iApply "Hclose". iNext. iExists #1. done.
 Restart.
   iIntros "HInv". rewrite /setone. ewp_pure_steps.
   rewrite /MyInv /inner.
   assert (H: Atomic StronglyAtomic (Store (LitV l) (LitV (Zpos xH)))).
-    by apply _.
+  1: by apply _.
   iApply (@ewp_atomic _ _ ⊤ (⊤ ∖ ↑invN) (Store (LitV l) (LitV (Zpos xH))) _ _ _ H). 
   iMod (inv_acc with "HInv") as "((%n & Hl) & Hclose)".
-  done.
+  1: done.
+  iModIntro.
+  iApply (ewp_store with "Hl").
+  iIntros "!> Hl !>".
+  iApply (fupd_elim (⊤ ∖ ↑invN) ⊤ ⊤ True True).
+  1: by iIntros "_ !>". 
+  iApply "Hclose". iNext. iExists #1. done.
+Restart.
+  iIntros "HInv". rewrite /setone. ewp_pure_steps.
+  rewrite /MyInv /inner.
+  assert (H: Atomic StronglyAtomic (Store (LitV l) (LitV (Zpos xH)))).
+  1: by apply _.
+  iApply (@ewp_atomic _ _ ⊤ (⊤ ∖ ↑invN) (Store (LitV l) (LitV (Zpos xH))) _ _ _ H). 
+  iMod (inv_acc with "HInv") as "((%n & Hl) & Hclose)".
+  1: done.
   iModIntro.
   iApply (ewp_store with "Hl").
   iIntros "!> Hl !>".
